Pom/Linearization.lean
@@ -6,22 +6,23 @@ open OmegaCompletePartialOrder Linearization
 namespace Pomfin
 
 noncomputable def lin (t : Type → Type) (α act test : Type)
-    [Linearizable t α] [Bot (t α)]
-    [Sem act α (t α)] [Sem test α (t Bool)]
+    [∀ β, OmegaCompletePartialOrder (t β)] [∀ β, OrderBot (t β)] [Linearizable t α]
+    [Preorder act] [Sem act α (t α)]
+    [Preorder test] [Sem test α (t Bool)]
     (p : Pomfin (Label act test)) : α → t α :=
   p.lift Lpofin.lin (fun _ _ ↦ Lpofin.lin_isomorphic)
 
 lemma lin_monotone (t : Type → Type) (α act test : Type)
-    [Linearizable t α]
-    [∀ {β : Type}, Preorder (t β)] [∀ {β : Type}, OrderBot (t β)]
+    [∀ β, OmegaCompletePartialOrder (t β)] [∀ β, OrderBot (t β)] [Linearizable t α]
     [PartialOrder act] [Sem act α (t α)]
     [PartialOrder test] [Sem test α (t Bool)] :
     Monotone (lin t α act test) :=
   Pomfin.lift_monotone Lpofin.lin_mono
 
 lemma lin_mk {t : Type → Type} {X act test : Type}
-    [Linearizable t X] [Bot (t X)]
-    [Sem act X (t X)] [Sem test X (t Bool)]
+    [∀ β, OmegaCompletePartialOrder (t β)] [∀ β, OrderBot (t β)] [Linearizable t X]
+    [Preorder act] [Sem act X (t X)]
+    [Preorder test] [Sem test X (t Bool)]
     (α : Lpofin (Label act test)) :
     lin t X act test (mk α) = Lpofin.lin α := by
   unfold lin; exact Quotient.lift_mk _ _ _
@@ -31,8 +32,7 @@ end Pomfin
 namespace Pom
 
 noncomputable def lin {t : Type → Type} {α act test : Type}
-    [Linearizable t α]
-    [∀ {β : Type}, OmegaCompletePartialOrder (t β)] [∀ {β : Type}, OrderBot (t β)]
+    [∀ β, OmegaCompletePartialOrder (t β)] [∀ β, OrderBot (t β)] [Linearizable t α]
     [DCPO act] [Sem act α (t α)]
     [DCPO test] [Sem test α (t Bool)]
     (p : Pom (Label act test)) : α → t α :=
@@ -41,24 +41,21 @@ noncomputable def lin {t : Type → Type} {α act test : Type}
 notation "𝓛" => lin
 
 lemma lin_continuous {t : Type → Type} {α act test : Type}
-    [Linearizable t α]
-    [∀ {β : Type}, OmegaCompletePartialOrder (t β)] [∀ {β : Type}, OrderBot (t β)]
+    [∀ β, OmegaCompletePartialOrder (t β)] [∀ β, OrderBot (t β)] [Linearizable t α]
     [DCPO act] [ScottCompact act] [Sem act α (t α)]
     [DCPO test] [ScottCompact test] [Sem test α (t Bool)] :
     ωScottContinuous (Pom.lin : Pom (Label act test) → α → t α) :=
   ext_continuous (Pomfin.lin_monotone t α act test)
 
 lemma lin_eq_fin {t : Type → Type} {α act test : Type}
-    [Linearizable t α]
-    [∀ {β : Type}, OmegaCompletePartialOrder (t β)] [∀ {β : Type}, OrderBot (t β)]
+    [∀ β, OmegaCompletePartialOrder (t β)] [∀ β, OrderBot (t β)] [Linearizable t α]
     [DCPO act] [Sem act α (t α)]
     [DCPO test] [Sem test α (t Bool)]
     (p : Pomfin (Label act test)) :
     lin p.to_pom = Pomfin.lin t α act test p := ext_eq_fin _ p
 
 lemma lin_mk {t : Type → Type} {X act test : Type}
-    [Linearizable t X]
-    [∀ {β : Type}, OmegaCompletePartialOrder (t β)] [∀ {β : Type}, OrderBot (t β)]
+    [∀ β, OmegaCompletePartialOrder (t β)] [∀ β, OrderBot (t β)] [Linearizable t X]
     [DCPO act] [Sem act X (t X)]
     [DCPO test] [Sem test X (t Bool)]
     (α : Lpo (Label act test)) :
