Pom/Linearization/Guard.lean
@@ -10,8 +10,8 @@ namespace Pom
 open OmegaCompletePartialOrder
 
 lemma lin_guard {t : Type → Type} {s act test : Type}
-    [Linearizable t s]
     [∀ {β : Type}, OmegaCompletePartialOrder (t β)] [∀ {β : Type}, OrderBot (t β)]
+    [Linearizable t s]
     [DCPO act] [ScottCompact act] [Sem act s (t s)]
     [DCPO test] [ScottCompact test] [Sem test s (t Bool)]
     (p q : Pom (Label act test)) (b : test) :
